src3.0/Transforms/phielim_top.v
@@ -7,142 +7,93 @@ Require Import primitives.
 Require Import die_wfS.
 Require Import die_top.
 Require Import subst.
+Require Import subst_sim.
+Require Import phielim_spec.
+Require Import phisubst_inv.
 
-Lemma eliminate_phi_false_spec: forall f p f'
-  (Helim: (f', false) = eliminate_phi f p), f = f'.
-Admitted.
-
-Lemma eliminate_phis_false_spec: forall f' f ps0
-  (Helim: (f', false) = eliminate_phis f ps0 ), f' = f.
-Proof.
-  induction ps0 as [|p]; simpl; intros.
-    congruence.
-
-    remember (eliminate_phi f p) as R.
-    destruct R as []; inv Helim.
-    destruct_if; auto.
-    apply eliminate_phi_false_spec in HeqR. subst. auto.
-Qed.
-
-(* vid = phi [vid vid ... vid] *)
-Inductive identity_phi: phinode -> Prop :=
-| identity_phi_intro: forall vid ty vls
-    (Hid: forall v0 l0, In (v0, l0) vls -> v0 = value_id vid),
-    identity_phi (insn_phi vid ty vls)
-.
-
-Lemma identity_phi_cannot_be_in_reachable_blocks: forall S M p f
-  l0 ps0 cs0 tmn0 (Hreach: reachable f l0) 
-  (Hwf: wf_fdef S M f) (Huniq: uniqFdef f)
-  (HBinF: blockInFdefB (block_intro l0 ps0 cs0 tmn0) f = true)
-  (Hin: In p ps0) (Hid: identity_phi p),
-  False. 
-Admitted.
-
-(* vid = phi [vid v ... vid v] *)
-Inductive assigned_phi (v:value): phinode -> Prop :=
-| assigned_phi_intro: forall vid ty vls
-    (Hex: exists l0, In (v, l0) vls)
-    (Hassign: forall v0 l0, In (v0, l0) vls -> v0 = value_id vid \/ v0 = v),
-    assigned_phi v (insn_phi vid ty vls)
-.
-
-Lemma assigned_phi__domination: forall S M p f l0 ps0 cs0 tmn0
-  (Hwf: wf_fdef S M f) (Huniq: uniqFdef f)
-  (HBinF: blockInFdefB (block_intro l0 ps0 cs0 tmn0) f = true) 
-  (Hin: In p ps0) v (Has: assigned_phi v p),
+Lemma subst_phi_init: forall (los : layouts) (nts : namedts) (fh : fheader)
+  (bs1 : list block) (l0 : l) (ps0 : phinodes) (cs0 : cmds) (tmn0 : terminator)
+  (bs2 : list block) (Ps1 : list product) (Ps2 : list product)
+  (v : value) p f
+  (Hin: In p ps0) (Hassign: assigned_phi v p)
+  (Heqf: f = fdef_intro fh (bs1 ++ block_intro l0 ps0 cs0 tmn0 :: bs2)) M
+  (HeqS: M = module_intro los nts (Ps1 ++ product_fdef f :: Ps2))
+  (HwfS : wf_system [M]),
+  blockInFdefB (block_intro l0 ps0 cs0 tmn0) f = true /\
+  wf_fdef [M] M f /\ uniqFdef f /\
   valueDominates f v (value_id (getPhiNodeID p)).
-Admitted.
-
-Lemma eliminate_phi_true_spec: forall S M f b f'
-  (Hreach: isReachableFromEntry f b) p 
-  (Hwf: wf_fdef S M f) (Huniq: uniqFdef f)
-  (HBinF: phinodeInFdefBlockB p f b = true)
-  (Helim: (f', true) = eliminate_phi f p),
-  exists v, assigned_phi v p /\ 
-    f' = remove_fdef (getPhiNodeID p) (subst_fdef (getPhiNodeID p) v f).
-Admitted.
-
-Lemma eliminate_phis_true_spec': forall f b f' S M 
-  (Hwf: wf_fdef S M f) (Huniq: uniqFdef f)
-  (Hreach: isReachableFromEntry f b) ps
-  (HBinF: forall p, In p ps -> phinodeInFdefBlockB p f b = true)
-  (Helim: (f', true) = eliminate_phis f ps),
-  exists p, In p ps /\ exists v, assigned_phi v p /\ 
-    f' = remove_fdef (getPhiNodeID p) (subst_fdef (getPhiNodeID p) v f).
 Proof.
-  induction ps as [|p]; simpl; intros.
-    inv Helim.
-
-    remember (eliminate_phi f p) as R.
-    destruct R as []; inv Helim.
-    destruct_if.
-      exists p.
-      split; auto. 
-      eapply eliminate_phi_true_spec in HeqR; eauto.
-
-      apply eliminate_phi_false_spec in HeqR. subst. 
-      apply IHps in H1; auto. 
-      destruct H1 as [p' [Hin [v [H1 H2]]]].
-      eauto 6.
-Qed.
-    
-Lemma eliminate_phis_true_spec: forall f f' l0 S M 
-  (Hwf: wf_fdef S M f) (Huniq: uniqFdef f)
-  (Hreach: reachable f l0) ps cs0 tmn0
-  (HBinF: blockInFdefB (block_intro l0 ps cs0 tmn0) f = true)
-  (Helim: (f', true) = eliminate_phis f ps),
-  exists p, In p ps /\ exists v, assigned_phi v p /\ 
-    f' = remove_fdef (getPhiNodeID p) (subst_fdef (getPhiNodeID p) v f).
-Proof.
-  intros.
-  eapply eliminate_phis_true_spec' with (b:=block_intro l0 ps cs0 tmn0); 
-    simpl; eauto 1.
-  intros.
-  bsplit; auto. simpl. solve_in_list.
+  intros. 
+  assert (blockInFdefB (block_intro l0 ps0 cs0 tmn0) f = true)
+    as HBinF.
+    rewrite Heqf. simpl. apply InBlocksB_middle.
+  assert (wf_fdef [module_intro los nts (Ps1++product_fdef f::Ps2)]
+          (module_intro los nts (Ps1++product_fdef f::Ps2)) 
+          f /\ uniqFdef f) as J.
+    subst.
+    apply wf_single_system__wf_uniq_fdef; auto.
+  destruct J as [HwfF HuniqF].
+  subst.
+  eapply assigned_phi__domination in Hassign; eauto.
 Qed.
 
-(* las_wfS.v should call this one *)
-Lemma subst_fdef_dom__diinfo: forall S M f id0 v0
-  (Hwf: wf_fdef S M f) (Huniq: uniqFdef f)
-  (Hpure: forall (instr : insn)
-            (Hlkup: lookupInsnViaIDFromFdef f id0 = ret instr),
-            die.pure_cmd instr)
-  (Hreach: id_in_reachable_block f id0)
-  (Hvdom: valueDominates f v0 (value_id id0)),
-  exists diinfo:die.DIInfo, 
-    die.DI_f diinfo = subst_fdef id0 v0 f /\ die.DI_id diinfo = id0.
+Lemma subst_phi_wfS: forall (los : layouts) (nts : namedts) (fh : fheader)
+  (bs1 : list block) (l0 : l) (ps0 : phinodes) (cs0 : cmds) (tmn0 : terminator)
+  (bs2 : list block) (Ps1 : list product) (Ps2 : list product)
+  (v : value) p f
+  (Hin: In p ps0) (Hassign: assigned_phi v p) M
+  (Heqf: f = fdef_intro fh (bs1 ++ block_intro l0 ps0 cs0 tmn0 :: bs2))
+  (HeqS: M = module_intro los nts (Ps1 ++ product_fdef f :: Ps2))
+  (HwfS : wf_system [M]),
+  wf_system 
+    [module_intro los nts
+      (Ps1 ++ product_fdef (subst_fdef (getPhiNodeID p) v f) :: Ps2)].
 Proof.
-  intros.
-  apply subst_fdef__diinfo; auto.
-    intro J.
-    destruct v0; simpl in *; try tauto.
-    destruct J as [J | J]; try tauto. subst.
-    eapply idDominates_acyclic; eauto.
-Qed.
+  intros. 
+  assert (Hinit:=HwfS).
+  eapply subst_phi_init in Hinit; eauto.
+  destruct Hinit as [J1 [J2 [J3 J4]]].
+  subst.
+  apply subst_wfS; auto.
+    apply lookupBlockViaIDFromFdef__notin_getArgsIDsOfFdef
+          with (b:=(block_intro l0 ps0 cs0 tmn0)); auto.     
+      apply inGetBlockIDs__lookupBlockViaIDFromFdef; auto.
+        simpl. xsolve_in_list. 
+     eapply assigned_phi__wf_value; eauto 1.
+Qed. 
 
-Lemma assigned_phi__wf_value: forall S M p f l0 ps0 cs0 tmn0
-  (Hwf: wf_fdef S M f) (Huniq: uniqFdef f)
-  (HBinF: blockInFdefB (block_intro l0 ps0 cs0 tmn0) f = true) 
-  (Hin: In p ps0) v (Hassign: assigned_phi v p),
-  forall ty, 
-    lookupTypViaIDFromFdef f (getPhiNodeID p) = Some ty ->
-    wf_value S M f v ty.
-Admitted.
-
-Lemma subst_sim: forall (los : layouts) (nts : namedts) (fh : fheader)
+Lemma subst_phi_sim: forall (los : layouts) (nts : namedts) (fh : fheader)
   (dones : list id) (main : id) (VarArgs : list (GVsT DGVs))
   (bs1 : list block) (l0 : l) (ps0 : phinodes) (cs0 : cmds) (tmn0 : terminator)
   (bs2 : list block) (Ps1 : list product) (Ps2 : list product)
-  (v : value) f i1 (Hdom: valueDominates f v (value_id i1))
-  S2 (Heq2: S2=[module_intro los nts
-                (Ps1 ++  product_fdef f :: Ps2)])
-  (Hok: defined_program S2 main VarArgs)
-  (HwfS : wf_system S2),
+  (v : value) p f
+  (Hin: In p ps0) (Hassign: assigned_phi v p) M
+  (Heqf: f = fdef_intro fh (bs1 ++ block_intro l0 ps0 cs0 tmn0 :: bs2))
+  (HeqS: M = module_intro los nts (Ps1 ++ product_fdef f :: Ps2))
+  (HwfS : wf_system [M])  (Hok: defined_program [M] main VarArgs),
   program_sim
-    [module_intro los nts (Ps1 ++ product_fdef (subst_fdef i1 v f) :: Ps2)]
-    S2 main VarArgs.
-Admitted.
+    [module_intro los nts 
+      (Ps1 ++ product_fdef (subst_fdef (getPhiNodeID p) v f) :: Ps2)]
+    [M] main VarArgs.
+Proof.
+  intros.
+  assert (Hinit:=HwfS).
+  eapply subst_phi_init in Hinit; eauto.
+  destruct Hinit as [J1 [J2 [J3 J4]]].
+  assert (lookupInsnViaIDFromFdef f (getPhiNodeID p) = Some (insn_phinode p))
+    as Hlkup.
+    eapply IngetPhiNodesIDs__lookupPhinodeViaIDFromFdef'; eauto.
+  set (pi:=mkPEInfo f p v Hlkup Hassign).
+  subst.
+  set (ctx_inv := fun (cfg:OpsemAux.Config) (St:@Opsem.State DGVs) => True).
+  apply SubstSim.sim with (ctx_inv:=ctx_inv); auto.
+    intros ? ? ? ? ? ? ? ? Hop ?. 
+    apply phisubst_inv.preservation with (pi:=pi) in Hop; auto.
+    intros ? ? ? ? ? ? Hinit. 
+    apply phisubst_inv.s_genInitState__inv with (pi:=pi) in Hinit; auto.
+    intros. subst. eapply subst_phi_wfS; eauto.
+    unfold ctx_inv. auto.
+Qed.
 
 Lemma eliminate_phis_sim_wfS: forall los nts Ps1 Ps2 rd,
  forall (fh : fheader) (efs : list id) (f1 : fdef) 
@@ -199,26 +150,20 @@ Proof.
       eapply die_wfS; eauto.
       eapply program_sim__preserves__defined_program in H0; eauto using die_sim.
 
-  Case "subse".
+  Case "subst".
     subst.
     split.
-      eapply subst_sim; eauto.
+      eapply subst_phi_sim; eauto.
     split.
-      apply subst_wfS; auto.
-        apply lookupBlockViaIDFromFdef__notin_getArgsIDsOfFdef
-          with (b:=(block_intro l0 ps0 cs0 tmn0)); auto.     
-          apply inGetBlockIDs__lookupBlockViaIDFromFdef; auto.
-            simpl. xsolve_in_list. 
-        eapply assigned_phi__wf_value; eauto.
-       
-      eapply program_sim__preserves__defined_program; eauto using subst_sim.
+      eapply subst_phi_wfS; eauto.
+      eapply program_sim__preserves__defined_program; eauto using subst_phi_sim.
 Qed.
 
 Lemma eliminate_phis_reachablity_successors: forall (f1 f2 : fdef) ps0,
  (f2, true) = eliminate_phis f1 ps0 ->
  reachablity_analysis f1 = reachablity_analysis f2 /\
  successors f1 = successors f2.
-Admitted.
+Admitted. (* reach succ  *)
 
 Ltac elimphi_tac :=
 intros;
