src3.0/Transforms/laa_top.v
@@ -10,6 +10,7 @@ Require Import primitives.
 Require Import palloca_props.
 Require Import alive_alloca.
 Require Import id_rhs_val.
+Require Import subst_inv.
 Require Import mem2reg.
 Require Import program_sim.
 Require Import memory_props.
@@ -17,582 +18,7 @@ Require Import trans_tactic.
 Require Import top_sim.
 Require Import laa.
 Require Import laa_wfS.
-
-(* same to las *)
-Lemma s_genInitState__laa_State_simulation: forall pinfo laainfo S1 S2 main
-  VarArgs cfg2 IS2
-  (Hssim: system_simulation pinfo laainfo S1 S2)
-  (Hinit: Opsem.s_genInitState S2 main VarArgs Mem.empty = ret (cfg2, IS2)),
-  exists cfg1, exists IS1,
-    Opsem.s_genInitState S1 main VarArgs Mem.empty = ret (cfg1, IS1) /\
-    State_simulation pinfo laainfo cfg1 IS1 cfg2 IS2.
-Proof.
-  unfold Opsem.s_genInitState.
-  intros.
-  inv_mbind'.
-  destruct m as [los nts ps].
-  inv_mbind'.
-  destruct b as [l0 ps0 cs0 tmn0].
-  destruct f as [[fa rt fid la va] bs].
-  inv_mbind'. symmetry_ctx.
-  assert (HlkF2FromS2:=HeqR).
-  eapply TopSim.system_simulation__fdef_simulation_r2l in HeqR; eauto.
-  destruct HeqR as [f1 [HlkF1fromS1 Hfsim]]. simpl in Hfsim.
-  fill_ctxhole.
-  eapply TopSim.system_simulation__getParentOfFdefFromSystem in HeqR0; eauto.
-  destruct HeqR0 as [m1 [J1 J2]].
-  fill_ctxhole. destruct m1 as [los1 nts1 ps1].
-  destruct J2 as [J2 [J3 J4]]; subst.
-  eapply TopSim.genGlobalAndInitMem_spec in HeqR1; eauto.
-  destruct HeqR1 as [gl1 [fs1 [M1 [HeqR1 [EQ1 [EQ2 EQ3]]]]]]; subst.
-  fill_ctxhole.
-  assert (J:=HeqR2).
-  eapply getEntryBlock__simulation in J; eauto.
-  destruct J as [b1 [J5 J6]].
-  fill_ctxhole.
-  destruct b1 as [l2 ps2 cs2 tmn2].
-  destruct f1 as [[fa1 rt1 fid1 la1 va1] bs1].
-  assert (J:=Hfsim).
-  apply fdef_simulation__eq_fheader in J.
-  inv J.
-  fill_ctxhole.
-  match goal with
-  | |- exists _:_, exists _:_, Some (?A, ?B) = _ /\ _ => exists A; exists B
-  end.
-  match goal with 
-  | H: getParentOfFdefFromSystem _ _ = _ |- _ =>
-    apply getParentOfFdefFromSystem__moduleInProductsInSystemB in H;
-    destruct H as [HMinS HinPs]
-  end.
-  assert (J:=J6).
-  apply block_simulation_inv in J.
-  destruct J as [J1 [J2 [J3 J7]]]; subst.
-  assert (blockInFdefB (block_intro l0 ps0 cs0 tmn0)
-           (fdef_intro (fheader_intro fa rt fid la va) bs) = true) as HBinF.
-    apply entryBlockInFdef; auto.
-  repeat (split; auto).
-    exists l0. exists ps2. exists nil. auto.
-    exists l0. exists ps0. exists nil. auto.
-Qed.
-
-(* same to las *)
-Lemma cmds_simulation_nil_inv' : forall (pinfo : PhiInfo) 
-  (laainfo : LAAInfo pinfo) (f1 : fdef) (cs : list cmd),
-  cmds_simulation pinfo laainfo f1 cs nil -> cs = nil.
-Proof.
-  unfold cmds_simulation. intros.
-  destruct_if; auto.
-    destruct cs; inv H1; auto.
-Qed.
-
-(* same to las *)
-Lemma cmds_simulation_cons_inv' : forall (pinfo : PhiInfo) 
-  (laainfo : LAAInfo pinfo) (f1 : fdef) (cs : list cmd) c2 cs2,
-  cmds_simulation pinfo laainfo f1 cs (c2::cs2) -> 
-  exists c1, exists cs1, 
-    cs = c1::cs1 /\
-    cmd_simulation pinfo laainfo f1 c1 c2 /\
-    cmds_simulation pinfo laainfo f1 cs1 cs2.
-Proof.
-  unfold cmds_simulation, cmd_simulation. intros.
-  destruct_if; eauto.
-    destruct cs; inv H1; eauto.
-Qed.
-
-(* same to las *)
-Inductive tmn_simulation' (pinfo:PhiInfo) (laainfo:LAAInfo pinfo) (F:fdef) 
-  : terminator -> terminator -> Prop :=
-| tmn_simulation_return : forall id0 t0 v v',
-    value_simulation pinfo laainfo F v v' ->
-    tmn_simulation' pinfo laainfo F (insn_return id0 t0 v) (insn_return id0 t0 v')
-| tmn_simulation_return_void : forall id0,
-    tmn_simulation' pinfo laainfo F (insn_return_void id0) (insn_return_void id0)
-| tmn_simulation_br : forall id0 v v' l1 l2,
-    value_simulation pinfo laainfo F v v' ->
-    tmn_simulation' pinfo laainfo F (insn_br id0 v l1 l2) (insn_br id0 v' l1 l2)
-| tmn_simulation_br_uncond : forall id0 l0,
-    tmn_simulation' pinfo laainfo F (insn_br_uncond id0 l0) 
-                                    (insn_br_uncond id0 l0)
-| tmn_simulation_unreachable : forall id0,
-    tmn_simulation' pinfo laainfo F (insn_unreachable id0) 
-                                    (insn_unreachable id0)
-.
-
-(* same to las *)
-Lemma tmn_simulation'__refl: forall pinfo laainfo F t,
-  PI_f pinfo <> F ->
-  tmn_simulation' pinfo laainfo F t t.
-Proof.
-  intros.
-  destruct t; constructor; auto using value_simulation__refl.
-Qed.
-
-(* same to las *)
-Lemma tmn_simulation__tmn_simulation': forall pinfo laainfo F t t'
-  (Htsim: tmn_simulation pinfo laainfo F t t'),
-  tmn_simulation' pinfo laainfo F t t'.
-Proof.
-  unfold tmn_simulation.
-  intros.
-  destruct (fdef_dec (PI_f pinfo) F); subst; auto using tmn_simulation'__refl.
-    destruct t; simpl;
-    constructor; try solve [
-      unfold value_simulation;
-      destruct (fdef_dec (PI_f pinfo) (PI_f pinfo)); try congruence; auto
-    ].
-Qed.
-
-(* same to las *)
-Ltac inTmnOp_isnt_stuck v H3 Hwfcfg1 Hwfpp1 :=
-match type of Hwfpp1 with
-| OpsemPP.wf_State 
-              {|
-              OpsemAux.CurSystem := _;
-              OpsemAux.CurTargetData := ?td;
-              OpsemAux.CurProducts := _;
-              OpsemAux.Globals := ?gl;
-              OpsemAux.FunTable := _ |}
-    {| Opsem.ECS := {| Opsem.CurFunction := _;
-                       Opsem.CurBB := ?b;
-                       Opsem.CurCmds := nil;
-                       Opsem.Terminator := ?tmn;
-                       Opsem.Locals := ?lc;
-                       Opsem.Allocas := _
-                     |} :: _;
-       Opsem.Mem := _ |}  =>
-    let G := fresh "G" in
-    let gvs := fresh "gvs" in
-    assert (exists gvs, Opsem.getOperandValue td v lc gl = Some gvs) as G; 
-      try solve [
-        destruct H3 as [l5 [ps2 [cs21 H3]]]; subst;
-        destruct Hwfcfg1 as [_ [Hwfg1 [Hwfs1 HmInS1]]];
-        destruct Hwfpp1 as 
-          [_ [[Hreach1 [HbInF1 [HfInPs1 [_ [Hinscope1 _]]]]] _]];
-        inv_mbind;
-        eapply OpsemPP.getOperandValue_inTmnOperans_isnt_stuck; eauto 1;
-          simpl; auto
-      ];
-    destruct G as [gvs G]
-end.
-
-(* same to las *)
-Ltac tmnOps_eq H3 Hwfcfg1 Hwfpp1 HwfS1 :=
-      destruct H3 as [l1 [ps1 [cs11 H3]]]; subst;
-      destruct Hwfcfg1 as [_ [Hwfg1 [Hwfs1 HmInS1]]];
-      destruct Hwfpp1 as [_ [[Hreach1 [HbInF1 [HfInPs1 [_ [Hinscope1 _]]]]] _]];
-      destruct HwfS1 as [HwfS1 _];
-      unfold wf_ExecutionContext, inscope_of_ec in HwfS1;
-      inv_mbind;
-      eapply getOperandValue_inTmnOperands_sim; 
-        eauto 2 using wf_system__wf_fdef, wf_system__uniqFdef; simpl; auto.
-
-(* same to las *)
-Lemma s_isFinialState__laa_State_simulation: forall
-  pinfo laainfo cfg1 FS1 cfg2 FS2
-  (Hwfcfg1: OpsemPP.wf_Config cfg1) (Hwfpp1: OpsemPP.wf_State cfg1 FS1) 
-  (Hwfcfg2: OpsemPP.wf_Config cfg2) (Hwfpp2: OpsemPP.wf_State cfg2 FS2) 
-  (HwfS1: id_rhs_val.wf_State (value_id (LAA_lid pinfo laainfo)) 
-           [! pinfo !] (PI_f pinfo) cfg1 FS1)
-  (Hstsim : State_simulation pinfo laainfo cfg1 FS1 cfg2 FS2),
-  Opsem.s_isFinialState cfg1 FS1 = Opsem.s_isFinialState cfg2 FS2.
-Proof.
-  unfold Opsem.s_isFinialState.
-  intros.
-  destruct cfg2 as [S2 [los2 nts2] gl2 fs2].
-  destruct cfg1 as [S1 [los1 nts1] gl1 fs1].
-  destruct FS1 as [[|[? ? cs1 ? ?] ES1]]; 
-  destruct FS2 as [[|[? ? cs2 ? ?] ES2]]; try solve [
-    auto |
-    destruct Hstsim as [X [? [Hstsim [? [? ?]]]]]; subst; inv Hstsim
-  ].
-  destruct Hstsim as [X [? [Hstsim [? [? ?]]]]]; subst.
-  inv X. simpl.
-  destruct Hstsim as [Hstsim Hstsim'].
-  fold ECs_simulation in Hstsim'.
-  destruct Hstsim as [? [Htmn [? [? [? [? [? Hstsim]]]]]]]; subst.
-  destruct cs1, cs2; try solve [
-    auto |
-    apply cmds_simulation_nil_inv in Hstsim; try congruence |
-    apply cmds_simulation_nil_inv' in Hstsim; try congruence
-  ].
-  apply tmn_simulation__tmn_simulation' in Htmn.
-  inv Htmn; auto.
-    destruct ES1, ES2; try solve [auto | inv Hstsim'].
-      inTmnOp_isnt_stuck v H3 Hwfcfg1 Hwfpp1.
-      inTmnOp_isnt_stuck v' H4 Hwfcfg2 Hwfpp2.
-      rewrite G. rewrite G0.
-      f_equal.
-      tmnOps_eq H3 Hwfcfg1 Hwfpp1 HwfS1.
-
-    destruct ES1, ES2; try solve [auto | inv Hstsim'].
-Qed.
-
-(* same to las *)
-Ltac undefined_state__State_simulation_r2l_tac1 :=
-  match goal with
-  | Hstsim: State_simulation _ _ _ ?St1 _ ?St2 |- _ =>
-    destruct St2 as [[|[? ? [|CurCmds] [] ?] [|[]]] ?]; try tauto;
-    destruct CurCmds; try tauto;
-    destruct St1 as [ECS ?];
-    destruct Hstsim as [X [? [Hstsim [? [? ?]]]]]; subst;
-    inv X;
-    destruct ECS as [|[] ECS]; try tauto;
-    destruct Hstsim as [Hstsim Hstsim'];
-    destruct ECS as [|[] ECS]; try tauto;
-    destruct Hstsim as [? [Htmn [? [? [? [? [? Hstsim]]]]]]]; subst;
-    destruct Hstsim' as [Hstsim' _];
-    destruct Hstsim' as [? [? [? [? [? [? [? Hstsim']]]]]]]; subst;
-   simpl
-  end.
-
-(* same to las *)
-Ltac undefined_state__State_simulation_r2l_tac3 :=
-  match goal with
-  | Hstsim: State_simulation _ _ _ ?St1 _ ?St2 |- _ =>
-    destruct St2 as [[|[? [? ? ? tmn] CurCmds tmn' ?] ?] ?]; try tauto;
-    destruct tmn; try tauto;
-    destruct CurCmds; try tauto;
-    destruct tmn'; try tauto;
-    destruct St1 as [ECS ?];
-    destruct Hstsim as [X [? [Hstsim [? [? H3]]]]]; subst;
-    inv X;
-    destruct ECS as [|[] ECS]; try tauto;
-    destruct Hstsim as [Hstsim _];
-    destruct Hstsim as [? [Htmn [? [? [? [? [? Hstsim]]]]]]]; subst;
-    let l5 := fresh "l5" in
-    destruct H3 as [l5 [ps5 [cs5 EQ]]]; subst
-  end.
-
-(* same to las *)
-Ltac undefined_state__State_simulation_r2l_tac41 :=
-  match goal with
-  | Hstsim: State_simulation _ _ _ ?St1 ?cfg2 ?St2 |- _ =>
-    destruct St1 as [ECS ?];
-    destruct Hstsim as [X [? [Hstsim [? [? ?]]]]]; subst;
-    inv X;
-    destruct ECS as [|[? ? ? ? Locals0] ECS]; try tauto;
-    destruct Hstsim as [Hstsim _];
-    destruct Hstsim as [? [? [? [? [H4 [H5 [? Hstsim]]]]]]]; subst
-  end. 
-
-(* same to las *)
-Ltac undefined_state__la_State_simulation_r2l_tac42 := 
-repeat match goal with
-| Hwfcfg1: OpsemPP.wf_Config ?cfg1, Hwfpp1: OpsemPP.wf_State ?cfg1 ?St1, 
-  HwfS1: wf_State _ _ _ ?cfg1 ?St1, 
-  Hvsim: value_simulation _ _ _ ?v0 ?v,
-  _: ret ?gn = Opsem.getOperandValue ?td ?v ?Locals ?fs2,
-  _: block_simulation _ _ _ ?b _,
-  H4: exists _:_, exists _:_, exists _:_, ?b = _ |- _ =>
-    let G := fresh "G" in
-    let gvs := fresh "gvs" in
-    assert (exists gvs, Opsem.getOperandValue td
-       v0 Locals fs2 = Some gvs) as G; try solve [
-      destruct H4 as [l5 [ps2 [cs21 H4]]]; subst;
-      destruct Hwfcfg1 as [_ [Hwfg1 [Hwfs1 HmInS1]]];
-      destruct Hwfpp1 as [_ [[Hreach1 [HbInF1 [HfInPs1 [_ [Hinscope1 _]]]]] _]];
-      inv_mbind;
-      eapply OpsemPP.getOperandValue_inCmdOps_isnt_stuck; eauto 1; simpl; auto
-    ];
-    destruct G as [gvs G];
-    assert (gvs = gn) as EQ; try solve [
-      destruct H4 as [l1 [ps1 [cs11 H4]]]; subst;
-      destruct Hwfcfg1 as [_ [Hwfg1 [Hwfs1 HmInS1]]];
-      destruct Hwfpp1 as [_ [[Hreach1 [HbInF1 [HfInPs1 [_ [Hinscope1 _]]]]] _]];
-      destruct HwfS1 as [HwfS1 _];
-      unfold wf_ExecutionContext, inscope_of_ec in HwfS1;
-      inv_mbind;
-      eapply getOperandValue_inCmdOperands_sim; 
-        eauto 2 using wf_system__wf_fdef, wf_system__uniqFdef; simpl; auto
-    ];
-    subst;
-    clear Hvsim
-end.
-
-(* same to las *)
-Ltac undefined_state__la_State_simulation_r2l_tac43 := 
-      match goal with
-      | Hstsim: cmds_simulation _ _ _ _ (_::_) |- _ =>
-      apply cmds_simulation_cons_inv' in Hstsim; subst;
-      destruct Hstsim as [c1' [cs2' [J1 [J2 J3]]]]; subst;
-      apply cmd_simulation__cmd_simulation' in J2;
-      inv J2;
-      undefined_state__la_State_simulation_r2l_tac42
-     end.
-
-(* same to las *)
-Lemma undefined_state__laa_State_simulation_r2l: forall pinfo laainfo cfg1 St1 
-  cfg2 St2 (Hstsim : State_simulation pinfo laainfo cfg1 St1 cfg2 St2)
-  (Hwfcfg1: OpsemPP.wf_Config cfg1) (Hwfpp1: OpsemPP.wf_State cfg1 St1) 
-  (HwfS1: id_rhs_val.wf_State (value_id (LAA_lid pinfo laainfo)) 
-           [! pinfo !] (PI_f pinfo) cfg1 St1)
-  (Hundef: OpsemPP.undefined_state cfg2 St2), OpsemPP.undefined_state cfg1 St1.
-Proof.
-  intros.
-  unfold OpsemPP.undefined_state in Hundef.
-  destruct cfg2 as [S2 [los2 nts2] gl2 fs2].
-  destruct cfg1 as [S1 [los1 nts1] gl1 fs1].
-  repeat match goal with
-  | Hundef : _ \/ _ |- _ => destruct Hundef as [Hundef | Hundef]
-  end.
-  Case "1".
-
-    undefined_state__State_simulation_r2l_tac1.
-    apply cmds_simulation_nil_inv' in Hstsim; subst.
-    apply cmds_simulation_cons_inv' in Hstsim'.
-    destruct Hstsim' as [c1' [cs1' [J1 [J2 J3]]]]; subst.
-    left. 
-    unfold tmn_simulation in Htmn. 
-    destruct_if; subst; simpl; auto.
-    match goal with
-    | H11: subst_tmn _ _ ?tmn = insn_return _ _ _ |- _ => 
-      destruct tmn; inv H11; auto
-    end.
-
-  Case "2".
-    undefined_state__State_simulation_r2l_tac1.
-    apply cmds_simulation_nil_inv' in Hstsim; subst.
-    apply cmds_simulation_cons_inv' in Hstsim'.
-    destruct Hstsim' as [c1' [cs1' [J1 [J2 J3]]]]; subst.
-    right. left.
-    assert (getCallerReturnID c = getCallerReturnID c1') as EQ.
-      unfold cmd_simulation in J2. subst. clear.
-      destruct_if; auto.
-      destruct c1'; auto.
-    rewrite <- EQ.
-    clear - Htmn Hundef.
-    unfold tmn_simulation in Htmn. 
-    destruct (fdef_dec (PI_f pinfo) CurFunction1); subst; simpl; auto.
-    match goal with
-    | H11: subst_tmn _ _ ?tmn = insn_return_void _ |- _ => 
-      destruct tmn; inv H11; auto
-    end.
-
-  Case "3".
-
-    undefined_state__State_simulation_r2l_tac3.
-    apply cmds_simulation_nil_inv' in Hstsim. subst.
-    right. right. left.
-    simpl. 
-    unfold tmn_simulation in Htmn. 
-    destruct_if; subst; simpl; auto.
-    match goal with
-    | H11: subst_tmn _ _ ?tmn = insn_unreachable _ |- _ => 
-      destruct tmn; inv H11; auto
-    end.
-
-  Case "4".
-
-    right; right; right; left;
-    destruct St2 as [[|[? ? [|[] CurCmds] tmn' Locals] ?] ?]; try solve [
-      tauto |
-
-      inv_mbind; destruct Hundef as [gn [EQ Hundef]]; inv EQ; inv_mbind;
-      undefined_state__State_simulation_r2l_tac41;
-      undefined_state__la_State_simulation_r2l_tac43;
-        repeat fill_ctxhole; exists gn; fill_ctxhole; auto
-    ].
-
-  Case "5".
-    right. right. right. right. left.
-    destruct St2 as [[|[? ? [|[] CurCmds] tmn' ?] ?] ?]; try tauto.
-    inv_mbind; destruct Hundef as [gn [EQ Hundef]]; inv EQ; inv_mbind.
-    undefined_state__State_simulation_r2l_tac41.
-    undefined_state__la_State_simulation_r2l_tac43.
-    repeat fill_ctxhole; exists gn; fill_ctxhole; auto.
-
-  Case "6".
-    right. right. right. right. right. left.
-    destruct St2 as [[|[? ? [|[] CurCmds] tmn' ?] ?] ?]; try tauto.
-    inv_mbind; destruct Hundef as [gvs [EQ Hundef]]; inv EQ; inv_mbind.
-    undefined_state__State_simulation_r2l_tac41.
-    undefined_state__la_State_simulation_r2l_tac43. 
-    repeat fill_ctxhole; exists gvs; fill_ctxhole; auto.
-
-  Case "7".
-    right. right. right. right. right. right. left.
-    destruct St2 as [[|[? ? [|[] CurCmds] tmn' ?] ?] ?]; try tauto.
-    inv_mbind; destruct Hundef as [gv [mgv [EQ1 [EQ2 Hundef]]]]; 
-      inv EQ1; inv EQ2; inv_mbind.
-    undefined_state__State_simulation_r2l_tac41.
-    undefined_state__la_State_simulation_r2l_tac43. 
-    repeat fill_ctxhole; exists gv; exists mgv; fill_ctxhole; auto.
-
-  Case "8".
-    destruct St2 as [[|[? ? [|[] CurCmds] tmn' ?] ?] ?]; try tauto.
-    right; right; right; right. right. right. right.
-    undefined_state__State_simulation_r2l_tac41.
-    inv_mbind.
-    destruct Hundef as [fptr [EQ Hundef]]; inv EQ.
-    inv_mbind.
-    apply cmds_simulation_cons_inv' in Hstsim; subst;
-    destruct Hstsim as [c1' [cs2' [J1 [J2 J3]]]]; subst.
-    apply cmd_simulation__cmd_simulation' in J2;
-    inv J2.  
-    undefined_state__la_State_simulation_r2l_tac42.
-    repeat fill_ctxhole.
-    exists fptr. split; auto.
-    remember (OpsemAux.lookupExFdecViaPtr gl2 FunTable fptr) as R.
-    destruct R as [[[]]|].
-      inv_mbind.
-      destruct Hundef as [gvs0 [EQ Hundef]].
-      dgvs_instantiate_inv.
-      assert (exists gvs, 
-                Opsem.params2GVs (los2,nts2) lp0 Locals fs2 = Some gvs) as G'.
-        destruct H4 as [l5 [ps2 [cs21 H4]]]; subst.
-        destruct Hwfcfg1 as [_ [Hwfg1 [Hwfs1 HmInS1]]];
-        destruct Hwfpp1 as [_ [[Hreach1 [HbInF1 [HfInPs1 [_ [Hinscope1 _]]]]] _]].
-        inv_mbind.
-        eapply OpsemPP.params2GVs_isnt_stuck; eauto 1; simpl; auto.
-          exists nil. auto.
-      destruct G' as [gvs' G'].
-      assert (gvs' = l1) as EQ.
-        destruct H4 as [l5 [ps1 [cs11 H4]]]; subst;
-        destruct Hwfcfg1 as [_ [Hwfg1 [Hwfs1 HmInS1]]];
-        destruct Hwfpp1 as [_ [[Hreach1 [HbInF1 [HfInPs1 [_ [Hinscope1 _]]]]] _]];
-        destruct HwfS1 as [HwfS1 _];
-        unfold wf_ExecutionContext, inscope_of_ec in HwfS1;
-        inv_mbind.
-        eapply params2GVs_sim; 
-          eauto 2 using wf_system__wf_fdef, wf_system__uniqFdef; 
-            try solve [simpl; auto].
-      subst.
-      repeat fill_ctxhole.
-      erewrite TopSim.lookupFdefViaPtr__simulation_None_l2r; eauto.
-      erewrite TopSim.lookupExFdecViaPtr__simulation_r2l; eauto.
-      simpl.
-      exists l1. split; auto.
-    
-      erewrite TopSim.lookupFdefViaPtr__simulation_None_l2r; eauto.
-      erewrite TopSim.lookupExFdecViaPtr__simulation_None_r2l; eauto.
-Qed.
-
-Lemma laa_is_bsim : forall pinfo laainfo Cfg1 St1 Cfg2 St2 St2' tr2 
-  (Hwfpi: WF_PhiInfo pinfo) 
-  (Hwfcfg: OpsemPP.wf_Config Cfg1) (Hwfpp: OpsemPP.wf_State Cfg1 St1) 
-  (Hwfcfg2: OpsemPP.wf_Config Cfg2) (Hwfpp2: OpsemPP.wf_State Cfg2 St2) 
-  (HwfS1: id_rhs_val.wf_State (value_id (LAA_lid pinfo laainfo)) 
-           [! pinfo !] (PI_f pinfo) Cfg1 St1)
-  (Hsim: State_simulation pinfo laainfo Cfg1 St1 Cfg2 St2)
-  (Hop2: Opsem.sInsn Cfg2 St2 St2' tr2)
-  (Hsubst: substable_values (OpsemAux.CurTargetData Cfg1) (OpsemAux.Globals Cfg1)
-             (PI_f pinfo) (value_id (LAA_lid pinfo laainfo))
-             [! pinfo !]) alinfo Hp
-  (Hlas2st : exist _ alinfo Hp = laainfo__alinfo pinfo laainfo)
-  (Halst: alive_alloca.wf_State pinfo alinfo Cfg1 St1)
-  (Hok: ~ sop_goeswrong Cfg1 St1),
-  exists St1', 
-    Opsem.sInsn Cfg1 St1 St1' tr2 /\
-    State_simulation pinfo laainfo Cfg1 St1' Cfg2 St2'.
-Proof.
-  intros.
-  assert (Hnfinal1: Opsem.s_isFinialState Cfg1 St1 = merror).
-    remember (Opsem.s_isFinialState Cfg1 St1) as R.
-    destruct R; auto.
-    apply s_isFinialState__laa_State_simulation in Hsim; 
-      try solve [auto | congruence].
-      contradict Hop2.
-      apply s_isFinialState__stuck. congruence.
-  assert (J:=Hwfpp).
-  apply OpsemPP.progress in J; auto.
-  destruct J as [Hfinal1 | [[IS1'' [tr0 Hop1]] | Hundef1]]; try congruence.
-    assert (OpsemPP.wf_State Cfg1 IS1'') as Hwfpp''.
-      apply OpsemPP.preservation in Hop1; auto.
-    assert (vev_State (value_id (LAA_lid pinfo laainfo))
-             [! pinfo !] (PI_f pinfo) Cfg1 St1) as Hvev.
-      eapply laa__alive_alloca__vev; eauto.
-    assert (id_rhs_val.wf_State (value_id (LAA_lid pinfo laainfo)) 
-           [! pinfo !] (PI_f pinfo) Cfg1 IS1'') as HwfS1'.
-      eapply id_rhs_val.preservation in Hop1; eauto.
-    eapply laa_is_sim in Hsim; eauto.
-    destruct Hsim as [Hsim EQ]; subst.
-    exists IS1''. 
-    split; eauto.
-
-    apply undefined_state__stuck' in Hundef1.
-    contradict Hok.
-    apply nonfinal_stuck_state_goes_wrong; auto.
-Qed.
-
-Lemma sop_star__laa_State_simulation: forall pinfo laainfo cfg1 IS1 cfg2 IS2 tr
-  FS2 (Hwfpi: WF_PhiInfo pinfo) 
-  (Hwfcfg1: OpsemPP.wf_Config cfg1) (Hwfcfg2: OpsemPP.wf_Config cfg2) 
-  (Hwfpp1: OpsemPP.wf_State cfg1 IS1) (Hwfpp2: OpsemPP.wf_State cfg2 IS2) 
-  (HwfS1: id_rhs_val.wf_State (value_id (LAA_lid pinfo laainfo)) 
-           [! pinfo !] (PI_f pinfo) cfg1 IS1) alinfo Hp
-  (Hsubst: substable_values (OpsemAux.CurTargetData cfg1) (OpsemAux.Globals cfg1)
-             (PI_f pinfo) (value_id (LAA_lid pinfo laainfo)) [! pinfo !])
-  (Hlas2st : exist _ alinfo Hp = laainfo__alinfo pinfo laainfo)
-  (Halst: alive_alloca.wf_State pinfo alinfo cfg1 IS1)
-  (Hstsim : State_simulation pinfo laainfo cfg1 IS1 cfg2 IS2) maxb
-  (Hless: 0 <= maxb) (Hwfgs: MemProps.wf_globals maxb (OpsemAux.Globals cfg1))
-  (Hnoalias: Promotability.wf_State maxb pinfo cfg1 IS1)
-  (Hstsim : State_simulation pinfo laainfo cfg1 IS1 cfg2 IS2)
-  (Hopstar : Opsem.sop_star cfg2 IS2 FS2 tr) (Hok: ~ sop_goeswrong cfg1 IS1),
-  exists FS1, Opsem.sop_star cfg1 IS1 FS1 tr /\
-    State_simulation pinfo laainfo cfg1 FS1 cfg2 FS2.
-Proof.
-  intros.
-  generalize dependent cfg1.
-  generalize dependent IS1.
-  induction Hopstar; intros.
-    exists IS1. split; auto.
-
-    eapply laa_is_bsim in Hstsim; eauto.
-    destruct Hstsim as [St1' [Hop1 Hstsim]].
-    assert (OpsemPP.wf_State cfg1 St1') as Hwfpp1'.
-      apply OpsemPP.preservation in Hop1; auto.
-    assert (vev_State (value_id (LAA_lid pinfo laainfo))
-             [! pinfo !] (PI_f pinfo) cfg1 IS1) as Hvev.
-      eapply laa__alive_alloca__vev; eauto.
-    assert (id_rhs_val.wf_State (value_id (LAA_lid pinfo laainfo))
-             [! pinfo !] (PI_f pinfo) cfg1 St1') as HwfS1'.
-      eapply id_rhs_val.preservation in Hop1; eauto.
-    assert (alive_alloca.wf_State pinfo alinfo cfg1 St1') as Halst'.
-      eapply alive_alloca.preservation in Hop1; eauto.
-    assert (Promotability.wf_State maxb pinfo cfg1 St1') as Hnoalias'.
-      eapply Promotability.preservation in Hop1; eauto.
-    eapply IHHopstar in Hstsim; 
-      eauto using sop_goeswrong__step, (@OpsemPP.preservation DGVs).
-    destruct Hstsim as [FS1 [Hopstar1 Hstsim]].
-    exists FS1.
-    split; eauto.
-Qed.
-
-Lemma sop_plus__laa_State_simulation: forall pinfo laainfo cfg1 IS1 cfg2 IS2 tr
-  FS2 (Hwfpi: WF_PhiInfo pinfo) 
-  (Hwfcfg1: OpsemPP.wf_Config cfg1) (Hwfcfg2: OpsemPP.wf_Config cfg2) 
-  (Hwfpp1: OpsemPP.wf_State cfg1 IS1) (Hwfpp2: OpsemPP.wf_State cfg2 IS2) 
-  (HwfS1: id_rhs_val.wf_State (value_id (LAA_lid pinfo laainfo)) 
-           [! pinfo !] (PI_f pinfo) cfg1 IS1) alinfo Hp
-  (Hsubst: substable_values (OpsemAux.CurTargetData cfg1) (OpsemAux.Globals cfg1)
-             (PI_f pinfo) (value_id (LAA_lid pinfo laainfo)) [! pinfo !])
-  (Hlas2st : exist _ alinfo Hp = laainfo__alinfo pinfo laainfo)
-  (Halst: alive_alloca.wf_State pinfo alinfo cfg1 IS1)
-  (Hstsim : State_simulation pinfo laainfo cfg1 IS1 cfg2 IS2) maxb
-  (Hless: 0 <= maxb) (Hwfgs: MemProps.wf_globals maxb (OpsemAux.Globals cfg1))
-  (Hnoalias: Promotability.wf_State maxb pinfo cfg1 IS1)
-  (Hstsim : State_simulation pinfo laainfo cfg1 IS1 cfg2 IS2)
-  (Hopplus : Opsem.sop_plus cfg2 IS2 FS2 tr) (Hok: ~ sop_goeswrong cfg1 IS1),
-  exists FS1, Opsem.sop_plus cfg1 IS1 FS1 tr /\
-    State_simulation pinfo laainfo cfg1 FS1 cfg2 FS2.
-Proof.
-  intros.
-  inv Hopplus.
-  eapply laa_is_bsim in Hstsim; eauto.
-  destruct Hstsim as [St1' [Hop1 Hstsim']].
-  assert (wf_State (value_id (LAA_lid pinfo laainfo)) [! pinfo !]
-     (PI_f pinfo) cfg1 St1') as HwfS1'.
-    eapply id_rhs_val.preservation in Hop1; eauto.
-      eapply laa__alive_alloca__vev; eauto.
-  eapply sop_star__laa_State_simulation in Hstsim'; eauto using
-    palloca_props.preservation, Promotability.preservation,
-    (@OpsemPP.preservation DGVs), sop_goeswrong__step,
-    alive_alloca.preservation.
-  destruct Hstsim' as [FS1 [Hopstar Hstsim']].
-  exists FS1. 
-  split; eauto.
-Qed.
+Require Import subst_sim.
 
 Lemma vev_State_preservation : forall pinfo laainfo cfg IS maxb
   (Hwfg: MemProps.wf_globals maxb (OpsemAux.Globals cfg))
@@ -610,80 +36,6 @@ Proof.
   eapply laa__alive_alloca__vev; eauto.
     apply OpsemPP.preservation in Hstep; auto.
     eapply alive_alloca.preservation in Hstep; eauto.
-Qed.
-
-Lemma id_rhs_val_preservation_star : forall v1 v2 F pinfo laainfo cfg IS IS' tr
-  (Heq1: v1 = value_id (LAA_lid pinfo laainfo))
-  (Heq2: v2 = [! pinfo !]) (Heq3: F = PI_f pinfo) maxb (Hle: 0 <= maxb)
-  (Hwfg: MemProps.wf_globals maxb (OpsemAux.Globals cfg))
-  (Halias: Promotability.wf_State maxb pinfo cfg IS) (Hwfpi: WF_PhiInfo pinfo)
-  alinfo Hp (Hlas2st : exist _ alinfo Hp = laainfo__alinfo pinfo laainfo)
-  (Halst: alive_alloca.wf_State pinfo alinfo cfg IS)
-  (Hvals : substable_values (OpsemAux.CurTargetData cfg) (OpsemAux.Globals cfg)
-             F v1 v2) (Hvev: vev_State v1 v2 F cfg IS) 
-  (Hwfcfg : OpsemPP.wf_Config cfg) (Hwfpp: OpsemPP.wf_State cfg IS) 
-  (HwfS1: id_rhs_val.wf_State v1 v2 F cfg IS) (Hstar: Opsem.sop_star cfg IS IS' tr),
-  id_rhs_val.wf_State v1 v2 F cfg IS'.
-Proof.
-  intros. subst.
-  induction Hstar; auto.
-    apply IHHstar; auto.
-      eapply Promotability.preservation; eauto.
-      eapply alive_alloca.preservation; eauto.
-      eapply OpsemPP.preservation; eauto.
-      eapply vev_State_preservation; eauto.
-      eapply id_rhs_val.preservation; eauto.
-Qed.  
-
-Lemma id_rhs_val_preservation_plus : forall v1 v2 F pinfo laainfo cfg IS IS' tr
-  (Heq1: v1 = value_id (LAA_lid pinfo laainfo))
-  (Heq2: v2 = [! pinfo !]) (Heq3: F = PI_f pinfo) maxb (Hle: 0 <= maxb)
-  (Hwfg: MemProps.wf_globals maxb (OpsemAux.Globals cfg))
-  (Halias: Promotability.wf_State maxb pinfo cfg IS) (Hwfpi: WF_PhiInfo pinfo)
-  alinfo Hp (Hlas2st : exist _ alinfo Hp = laainfo__alinfo pinfo laainfo)
-  (Halst: alive_alloca.wf_State pinfo alinfo cfg IS)
-  (Hvals : substable_values (OpsemAux.CurTargetData cfg) (OpsemAux.Globals cfg)
-             F v1 v2) (Hvev: vev_State v1 v2 F cfg IS) 
-  (Hwfcfg : OpsemPP.wf_Config cfg) (Hwfpp: OpsemPP.wf_State cfg IS) 
-  (HwfS1: id_rhs_val.wf_State v1 v2 F cfg IS) (Hplus: Opsem.sop_plus cfg IS IS' tr),
-  id_rhs_val.wf_State v1 v2 F cfg IS'.
-Proof.
-  intros.
-  apply OpsemProps.sop_plus__implies__sop_star in Hplus.
-  eapply id_rhs_val_preservation_star; eauto.
-Qed.
-
-Lemma sop_div__laa_State_simulation: forall pinfo laainfo cfg1 IS1 cfg2 IS2 tr
-  (Hwfpi: WF_PhiInfo pinfo)
-  (Hwfcfg1: OpsemPP.wf_Config cfg1) (Hwfcfg2: OpsemPP.wf_Config cfg2) 
-  (Hwfpp1: OpsemPP.wf_State cfg1 IS1) (Hwfpp2: OpsemPP.wf_State cfg2 IS2) 
-  (HwfS1: id_rhs_val.wf_State (value_id (LAA_lid pinfo laainfo)) 
-            [! pinfo !] (PI_f pinfo) cfg1 IS1) alinfo Hp
-  (Hsubst: substable_values (OpsemAux.CurTargetData cfg1) (OpsemAux.Globals cfg1)
-             (PI_f pinfo) (value_id (LAA_lid pinfo laainfo)) [! pinfo !])
-  (Hlas2st : exist _ alinfo Hp = laainfo__alinfo pinfo laainfo)
-  (Halst: alive_alloca.wf_State pinfo alinfo cfg1 IS1)
-  (Hstsim : State_simulation pinfo laainfo cfg1 IS1 cfg2 IS2) maxb
-  (Hless: 0 <= maxb) (Hwfgs: MemProps.wf_globals maxb (OpsemAux.Globals cfg1))
-  (Hnoalias: Promotability.wf_State maxb pinfo cfg1 IS1)
-  (Hstsim : State_simulation pinfo laainfo cfg1 IS1 cfg2 IS2)
-  (Hdiv : Opsem.sop_diverges cfg2 IS2 tr) (Hok: ~ sop_goeswrong cfg1 IS1),
-  Opsem.sop_diverges cfg1 IS1 tr.
-Proof.
-  cofix CIH.
-  intros.
-  inv Hdiv.
-  eapply sop_plus__laa_State_simulation in Hstsim; eauto 1.
-  destruct Hstsim as [FS1 [Hopplus Hstsim']].
-  econstructor; eauto.
-  assert (wf_State (value_id (LAA_lid pinfo laainfo)) [! pinfo !]
-     (PI_f pinfo) cfg1 FS1) as HwfS1'.
-    eapply id_rhs_val_preservation_plus; eauto.
-      eapply laa__alive_alloca__vev; eauto.
-  eapply CIH in Hstsim'; eauto using
-    palloca_props.preservation_plus, Promotability.preservation_plus,
-    (@OpsemPP.preservation_plus DGVs), sop_goeswrong__plus,
-    alive_alloca.preservation_plus.
 Qed.
 
 Lemma LAA_value__dominates__LAA_lid: forall pinfo lasinfo,
@@ -728,7 +80,7 @@ Lemma laa_sim: forall (los : layouts) (nts : namedts) (fh : fheader)
          :: Ps2)]
      S2 main VarArgs.
 Proof.
-  intros.
+  intros. subst.
   assert (blockInFdefB (block_intro l0 ps0 cs0 tmn0) (PI_f pinfo) = true)
     as HBinF.
     rewrite Heq. simpl. apply InBlocksB_middle.
@@ -740,121 +92,59 @@ Proof.
   destruct J as [HwfF HuniqF].
   eapply find_st_ld__laainfo in HBinF; eauto.
   destruct HBinF as [EQ [laainfo [J1 J2]]]; subst.
-  assert (Huniq:=HwfS). apply wf_system__uniqSystem in Huniq; auto.
-  assert (system_simulation pinfo laainfo
-     [module_intro los nts
-        (Ps1 ++
-         product_fdef
-           (fdef_intro fh (bs1 ++ block_intro l0 ps0 cs0 tmn0 :: bs2)) :: Ps2)]
-     [module_intro los nts
-        (Ps1 ++
-         product_fdef
-           (subst_fdef (LAA_lid pinfo laainfo) [! pinfo !]
-              (fdef_intro fh (bs1 ++ block_intro l0 ps0 cs0 tmn0 :: bs2)))
-         :: Ps2)]) as Hssim.
-    constructor; auto.
-    repeat split; auto.
-    simpl in Huniq. destruct Huniq as [[_ [_ Huniq]] _].
-    unfold TopSim.products_simulation. unfold fsim. unfold Fsim. 
-    apply uniq_products_simulation; auto.
+  set (ctx_inv := fun cfg IS =>
+    exists maxb, exists stinfo, exists Hp, 
+      0 <= maxb /\
+      MemProps.wf_globals maxb (OpsemAux.Globals cfg) /\
+      Promotability.wf_State maxb pinfo cfg IS /\ WF_PhiInfo pinfo /\
+      (exist _ stinfo Hp = laainfo__alinfo pinfo laainfo) /\
+      (alive_alloca.wf_State pinfo stinfo cfg IS) /\
+      (substable_values (OpsemAux.CurTargetData cfg) (OpsemAux.Globals cfg)
+         (PI_f pinfo) (value_id (LAA_lid pinfo laainfo)) [! pinfo !]) /\ 
+      (vev_State (value_id (LAA_lid pinfo laainfo)) [! pinfo !]
+         (PI_f pinfo) cfg IS)).
+  apply SubstSim.sim with (ctx_inv:=ctx_inv); auto.
+    intros. 
+    rewrite <- Heq in *. 
+    destruct Hp as [maxb [stinfo [Hp [G1 [G2 [G3 [G4 [G5 [G6 [G7 G8]]]]]]]]]].
+    eapply id_rhs_val.preservation; eauto.
+  
+    intros.
+    destruct H2 as [maxb [stinfo [Hp [G1 [G2 [G3 [G4 [G5 [G6 [G7 G8]]]]]]]]]].
+    exists maxb. exists stinfo. exists Hp. 
+    repeat (split; auto).
+      eapply Promotability.preservation; eauto.
+      eapply alive_alloca.preservation; eauto.
+      eapply vev_State_preservation; eauto.
 
-Ltac laa_sim_init :=
-match goal with
-| H: Opsem.s_genInitState [module_intro ?los ?nts _] _ _ _ = Some (?cfg, ?IS),  
-  pinfo: PhiInfo, laainfo: LAAInfo _
-  |- _ =>
+    intros.
+    rewrite <- Heq in *.  
+    eapply s_genInitState__id_rhs_val; eauto.
+      destruct cfg. simpl.
+      eapply LAA_substable_values; eauto.
+
+    intros. subst.
+    eapply laa_wfS; eauto.
+
+    intros.
+    rewrite <- Heq in *.  
     assert (OpsemPP.wf_Config cfg /\ OpsemPP.wf_State cfg IS) as Hwfst';
-      try solve [eapply s_genInitState__opsem_wf in H; eauto using laa_wfS];
-    eapply s_genInitState__laa_State_simulation in H; eauto;
-    destruct H as [cfg1 [IS1 [Hinit Hstsim]]];
-    assert (OpsemPP.wf_Config cfg1 /\ OpsemPP.wf_State cfg1 IS1) as Hwfst;
-      try solve [eapply s_genInitState__opsem_wf; eauto];
-    assert (id_rhs_val.wf_State (value_id (LAA_lid pinfo laainfo))
-              [! pinfo !] (PI_f pinfo) cfg1 IS1) as Hisrhsval;
-      try solve [eapply s_genInitState__id_rhs_val; 
-                 eauto using LAA_substable_values];
+      try solve [eapply s_genInitState__opsem_wf in H; eauto using laa_wfS].
+    assert (substable_values (OpsemAux.CurTargetData cfg) (OpsemAux.Globals cfg)
+      (PI_f pinfo) (value_id (LAA_lid pinfo laainfo)) [! pinfo !]) 
+      as Hdom.
+      destruct cfg. simpl.
+      eapply LAA_substable_values; eauto.
     assert (exists maxb,
-              MemProps.wf_globals maxb (OpsemAux.Globals cfg1) /\ 0 <= maxb /\
-              Promotability.wf_State maxb pinfo cfg1 IS1) as Hprom;
-      try solve [eapply Promotability.s_genInitState__wf_globals_promotable; eauto];
-    destruct Hprom as [maxb [Hwfg [Hless Hprom]]];
-    remember (laainfo__alinfo pinfo laainfo) as R;
-    destruct R as [alinfo Hp];
-    assert (substable_values (OpsemAux.CurTargetData cfg1) (OpsemAux.Globals cfg1)
-      (PI_f pinfo) (value_id (LAA_lid pinfo laainfo)) [! pinfo !]) as Hdom;
-      try solve [
-      assert ((los,nts) = OpsemAux.CurTargetData cfg1) as EQ;
-        try solve [eapply s_genInitState__targedata; eauto];
-      rewrite <- EQ;
-      eapply LAA_substable_values; eauto
-     ];
-    assert (alive_alloca.wf_State pinfo alinfo cfg1 IS1) as Halst;
-      try solve [eapply s_genInitState__alive_alloca; eauto]
-end.
-
-Ltac laa_sim_end :=
- match goal with
-| Hstsim' : State_simulation ?pinfo ?laainfo ?cfg1 ?FS1 ?cfg ?FS,
-  Hopstar1 : Opsem.sop_star ?cfg1 _ ?FS1 _ |- _ =>
-    assert (OpsemPP.wf_State cfg FS) as Hwfst''; 
-      try solve [eapply OpsemPP.preservation_star; eauto; try tauto];
-    assert (OpsemPP.wf_State cfg1 FS1) as Hwfst1'';
-      try solve [eapply OpsemPP.preservation_star; eauto; try tauto];
-    assert (wf_State (value_id (LAA_lid pinfo laainfo)) [! pinfo !]
-      (PI_f pinfo) cfg1 FS1); try solve [
-      eapply id_rhs_val_preservation_star in Hopstar1; eauto; try solve [
-        tauto |
-        eapply laa__alive_alloca__vev; eauto; try tauto
-      ]
-    ]
-end.
-
-  constructor; auto.
-    intros tr t Hconv.
-    inv Hconv.
-    laa_sim_init.
-    eapply sop_star__laa_State_simulation in Hstsim; 
-      eauto using defined_program__doesnt__go_wrong; try tauto.
-    destruct Hstsim as [FS1 [Hopstar1 Hstsim']].
-    laa_sim_end.
-    match goal with
-    | Hstsim' : State_simulation _ _ _ _ ?cfg ?FS,
-      H: Opsem.s_isFinialState ?cfg ?FS = _ |- _ =>
-      eapply s_isFinialState__laa_State_simulation in Hstsim'; eauto; try tauto;
-      rewrite <- Hstsim' in H
-    end.
-    exists t. split; auto using result_match_relf. econstructor; eauto.
-
-    intros tr Hdiv.
-    inv Hdiv.
-    laa_sim_init.
-    eapply sop_div__laa_State_simulation in Hstsim; 
-      eauto using defined_program__doesnt__go_wrong; try tauto.
-    destruct Hstsim as [FS1 Hopdiv1].
-    econstructor; eauto.
-
-    intros tr t Hgowrong.
-    inv Hgowrong.
-    assert (OpsemPP.wf_Config cfg /\ OpsemPP.wf_State cfg t) as HwfSt.
-      eapply s_genInitState__opsem_wf in H; eauto using laa_wfS.
-      destruct H as [Hcfg2 HwfSt2].
-      apply OpsemPP.preservation_star in H0; auto.
-    assert (OpsemPP.undefined_state cfg t) as Hundef.
-      apply stuck__undefined_state in H2; try solve [auto | tauto].
-    laa_sim_init.
-    eapply sop_star__laa_State_simulation in Hstsim;
-      eauto using defined_program__doesnt__go_wrong; try tauto.
-    destruct Hstsim as [FS1 [Hopstar1 Hstsim']].
-    assert (Hprom':=Hprom).
-    eapply Promotability.preservation_star in Hprom'; eauto; try tauto.
-    laa_sim_end.
-    assert (OpsemPP.undefined_state cfg1 FS1) as Hundef'.
-      eapply undefined_state__laa_State_simulation_r2l in Hundef; 
-        try solve [eauto | tauto].
-    assert (Opsem.s_isFinialState cfg1 FS1 = merror) as Hfinal'.
-      erewrite <- s_isFinialState__laa_State_simulation in H2; 
-        try solve [eauto | tauto].
-    apply undefined_state__stuck' in Hundef'.
-    exists tr. exists FS1.
-    econstructor; eauto.
+              MemProps.wf_globals maxb (OpsemAux.Globals cfg) /\ 0 <= maxb /\
+              Promotability.wf_State maxb pinfo cfg IS) as Hprom;
+      try solve [eapply Promotability.s_genInitState__wf_globals_promotable; eauto].
+    destruct Hprom as [maxb [Hwfg [Hless Hprom]]].
+    remember (laainfo__alinfo pinfo laainfo) as R.
+    destruct R as [stinfo Hp].
+    assert (alive_alloca.wf_State pinfo stinfo cfg IS) as Halst;
+      try solve [eapply s_genInitState__alive_alloca; eauto].
+    exists maxb. exists stinfo. exists Hp.
+    repeat (split; auto).
+      eapply laa__alive_alloca__vev; eauto; try tauto.
 Qed.
