src3.0/Transforms/phielim_spec.v
@@ -1,0 +1,106 @@
+Require Import vellvm.
+Require Import primitives.
+Require Import mem2reg.
+
+Lemma eliminate_phi_false_spec: forall f p f'
+  (Helim: (f', false) = eliminate_phi f p), f = f'.
+Admitted. (* spec *)
+
+Lemma eliminate_phis_false_spec: forall f' f ps0
+  (Helim: (f', false) = eliminate_phis f ps0 ), f' = f.
+Proof.
+  induction ps0 as [|p]; simpl; intros.
+    congruence.
+
+    remember (eliminate_phi f p) as R.
+    destruct R as []; inv Helim.
+    destruct_if; auto.
+    apply eliminate_phi_false_spec in HeqR. subst. auto.
+Qed.
+
+(* vid = phi [vid vid ... vid] *)
+Inductive identity_phi: phinode -> Prop :=
+| identity_phi_intro: forall vid ty vls
+    (Hid: forall v0 l0, In (v0, l0) vls -> v0 = value_id vid),
+    identity_phi (insn_phi vid ty vls)
+.
+
+Lemma identity_phi_cannot_be_in_reachable_blocks: forall S M p f
+  l0 ps0 cs0 tmn0 (Hreach: reachable f l0) 
+  (Hwf: wf_fdef S M f) (Huniq: uniqFdef f)
+  (HBinF: blockInFdefB (block_intro l0 ps0 cs0 tmn0) f = true)
+  (Hin: In p ps0) (Hid: identity_phi p),
+  False. 
+Admitted. (* dom *)
+
+(* vid = phi [vid v ... vid v] *)
+Inductive assigned_phi (v:value): phinode -> Prop :=
+| assigned_phi_intro: forall vid ty vls
+    (Hex: exists l0, In (v, l0) vls)
+    (Hassign: forall v0 l0, In (v0, l0) vls -> v0 = value_id vid \/ v0 = v),
+    assigned_phi v (insn_phi vid ty vls)
+.
+
+Lemma assigned_phi__domination: forall S M p f l0 ps0 cs0 tmn0
+  (Hwf: wf_fdef S M f) (Huniq: uniqFdef f)
+  (HBinF: blockInFdefB (block_intro l0 ps0 cs0 tmn0) f = true) 
+  (Hin: In p ps0) v (Has: assigned_phi v p),
+  valueDominates f v (value_id (getPhiNodeID p)).
+Admitted. (* dom *)
+
+Lemma eliminate_phi_true_spec: forall S M f b f'
+  (Hreach: isReachableFromEntry f b) p 
+  (Hwf: wf_fdef S M f) (Huniq: uniqFdef f)
+  (HBinF: phinodeInFdefBlockB p f b = true)
+  (Helim: (f', true) = eliminate_phi f p),
+  exists v, assigned_phi v p /\ 
+    f' = remove_fdef (getPhiNodeID p) (subst_fdef (getPhiNodeID p) v f).
+Admitted. (* spec *)
+
+Lemma eliminate_phis_true_spec': forall f b f' S M 
+  (Hwf: wf_fdef S M f) (Huniq: uniqFdef f)
+  (Hreach: isReachableFromEntry f b) ps
+  (HBinF: forall p, In p ps -> phinodeInFdefBlockB p f b = true)
+  (Helim: (f', true) = eliminate_phis f ps),
+  exists p, In p ps /\ exists v, assigned_phi v p /\ 
+    f' = remove_fdef (getPhiNodeID p) (subst_fdef (getPhiNodeID p) v f).
+Proof.
+  induction ps as [|p]; simpl; intros.
+    inv Helim.
+
+    remember (eliminate_phi f p) as R.
+    destruct R as []; inv Helim.
+    destruct_if.
+      exists p.
+      split; auto. 
+      eapply eliminate_phi_true_spec in HeqR; eauto.
+
+      apply eliminate_phi_false_spec in HeqR. subst. 
+      apply IHps in H1; auto. 
+      destruct H1 as [p' [Hin [v [H1 H2]]]].
+      eauto 6.
+Qed.
+    
+Lemma eliminate_phis_true_spec: forall f f' l0 S M 
+  (Hwf: wf_fdef S M f) (Huniq: uniqFdef f)
+  (Hreach: reachable f l0) ps cs0 tmn0
+  (HBinF: blockInFdefB (block_intro l0 ps cs0 tmn0) f = true)
+  (Helim: (f', true) = eliminate_phis f ps),
+  exists p, In p ps /\ exists v, assigned_phi v p /\ 
+    f' = remove_fdef (getPhiNodeID p) (subst_fdef (getPhiNodeID p) v f).
+Proof.
+  intros.
+  eapply eliminate_phis_true_spec' with (b:=block_intro l0 ps cs0 tmn0); 
+    simpl; eauto 1.
+  intros.
+  bsplit; auto. simpl. solve_in_list.
+Qed.
+
+Lemma assigned_phi__wf_value: forall S M p f l0 ps0 cs0 tmn0
+  (Hwf: wf_fdef S M f) (Huniq: uniqFdef f)
+  (HBinF: blockInFdefB (block_intro l0 ps0 cs0 tmn0) f = true) 
+  (Hin: In p ps0) v (Hassign: assigned_phi v p),
+  forall ty, 
+    lookupTypViaIDFromFdef f (getPhiNodeID p) = Some ty ->
+    wf_value S M f v ty.
+Admitted. (* spec *)
