src3.0/Transforms/phisubst_inv.v
@@ -1,0 +1,30 @@
+Require Import vellvm.
+Require Import primitives.
+Require Import subst_inv.
+Require Import phielim_spec.
+
+Record PEInfo := mkPEInfo {
+  PEI_f : fdef;
+  PEI_p : phinode;
+  PEI_v : value;
+  PEI_lkup: lookupInsnViaIDFromFdef PEI_f (getPhiNodeID PEI_p) = 
+              Some (insn_phinode PEI_p);
+  PEI_assign: assigned_phi PEI_v PEI_p
+}.
+
+Lemma preservation: forall (cfg1 : OpsemAux.Config)
+  (S1 S1' : Opsem.State) (tr : trace) (pi: PEInfo)
+  (Hcfg: OpsemPP.wf_Config cfg1) (Hpp: OpsemPP.wf_State cfg1 S1)
+  (Hop: Opsem.sInsn cfg1 S1 S1' tr)
+  (HwfS : subst_inv.wf_State (value_id (getPhiNodeID (PEI_p pi))) (PEI_v pi) 
+          (PEI_f pi) cfg1 S1),
+  subst_inv.wf_State (value_id (getPhiNodeID (PEI_p pi))) (PEI_v pi) (PEI_f pi) 
+    cfg1 S1'.
+Admitted.
+
+Lemma s_genInitState__inv: forall (S : system) (main : id) (pi: PEInfo) 
+  (VarArgs : list (GVsT DGVs)) (cfg : OpsemAux.Config) (IS : Opsem.State)
+  (HwfS: wf_system S)
+  (Hinit: Opsem.s_genInitState S main VarArgs Mem.empty = ret (cfg, IS)),
+  wf_State (value_id (getPhiNodeID (PEI_p pi))) (PEI_v pi) (PEI_f pi) cfg IS.
+Admitted.
