src3.0/Transforms/subst_inv.v
@@ -1,0 +1,55 @@
+Require Import vellvm.
+Require Import Lattice.
+
+Definition DGVMap := @Opsem.GVsMap DGVs.
+
+(* The invariant is fine to prove subst v1 by v2 in f when v2 >> v1.
+   when value_in_scope v1 ids0, we must have value_in_scope v2 ids0. 
+*)
+Definition wf_defs (v1 v2:value) F TD gl (f:fdef) (lc:DGVMap) ids0: Prop :=
+F = f ->
+forall gvs1 gvs2,
+  value_in_scope v1 ids0 ->
+  Opsem.getOperandValue TD v1 lc gl = Some gvs1 ->
+  Opsem.getOperandValue TD v2 lc gl = Some gvs2 ->
+  gvs1 = gvs2.
+
+Definition inscope_of_ec (ec:@Opsem.ExecutionContext DGVs) : option ids :=
+let '(Opsem.mkEC f b cs tmn lc als) := ec in
+match cs with
+| nil => inscope_of_tmn f b tmn
+| c::_ => inscope_of_cmd f b c
+end.
+
+Definition wf_ExecutionContext v1 v2 F TD gl (ps:list product)
+  (ec:Opsem.ExecutionContext) : Prop :=
+match inscope_of_ec ec with
+| Some ids0 =>
+    wf_defs v1 v2 F TD gl (Opsem.CurFunction ec) (Opsem.Locals ec) ids0
+| _ => False
+end.
+
+Fixpoint wf_ECStack v1 v2 F TD gl (ps:list product) (ecs:Opsem.ECStack) : Prop :=
+match ecs with
+| nil => True
+| ec::ecs' =>
+    wf_ExecutionContext v1 v2 F TD gl ps ec /\ wf_ECStack v1 v2 F TD gl ps ecs'
+end.
+
+Definition wf_State v1 v2 F (cfg:OpsemAux.Config) (S:Opsem.State) : Prop :=
+let '(OpsemAux.mkCfg s td ps gl _ ) := cfg in
+let '(Opsem.mkState ecs _) := S in
+wf_ECStack v1 v2 F td gl ps ecs.
+
+Lemma wf_defs_eq : forall ids2 ids1 v1 v2 F td gl F' lc',
+  AtomSet.set_eq _ ids1 ids2 ->
+  wf_defs v1 v2 F td gl F' lc' ids1 ->
+  wf_defs v1 v2 F td gl F' lc' ids2.
+Proof.
+  intros.
+  intros EQ gv1 gv2 Hin1 Hget1 Hget2; subst.
+  destruct H as [J1 J2].
+  eapply H0; eauto.
+    destruct v1; simpl in *; eauto.
+Qed.
+
